Tap

Gt3/JEq/Basic.lean
@@ -3,60 +3,63 @@ import Gt3.Ctx
 inductive Ctx.JEq : Ctx → Tm 0 → Tm 0 → Tm 0 → Prop
   -- Congruence rules
   | fv {Γ : Ctx} {x : String} {A : Tm 0}
-  (hΓ : JEq Γ .unit .null .null)
-  (hx : Ctx.Lookup Γ x A)
-  : JEq Γ A (Tm.fv x) (Tm.fv x)
-  | univ {Γ : Ctx} {ℓ ℓ'} (h : ℓ < ℓ')
-  : JEq Γ .unit .null .null → JEq Γ (.univ ℓ') (.univ ℓ) (.univ ℓ)
+    (hΓ : JEq Γ .unit .null .null)
+    (hx : Ctx.Lookup Γ x A)
+    : JEq Γ A (Tm.fv x) (Tm.fv x)
+  | univ {Γ : Ctx} {ℓ}
+    : JEq Γ .unit .null .null → JEq Γ (.univ (ℓ + 1)) (.univ ℓ) (.univ ℓ)
   | empty {Γ : Ctx} {ℓ} : JEq Γ .unit .null .null → JEq Γ (.univ ℓ) .empty .empty
   | unit {Γ : Ctx} {ℓ} : JEq Γ .unit .null .null → JEq Γ (.univ ℓ) .unit .unit
-  | eqn {Γ : Ctx} {A a a' b b' : Tm 0}
-  (ha : JEq Γ A a a')
-  (hb : JEq Γ A b b')
-  : JEq Γ (.univ 0) (.eqn a b) (.eqn a' b')
+  | eqn {Γ : Ctx} {A a a' b b' : Tm 0} {ℓ : ℕ}
+    (ha : JEq Γ A a a')
+    (hb : JEq Γ A b b')
+    : JEq Γ (.univ ℓ) (.eqn a b) (.eqn a' b')
   | pi {Γ : Ctx} {A A' : Tm 0} {B B' : Tm 1} {ℓ m n : ℕ} {L : Finset String}
-  (hA : JEq Γ (.univ m) A A')
-  (hB : ∀ x ∉ L, JEq (Γ.cons x A) (.univ n) (B.open x) (B'.open x))
-  (hm : m ≤ ℓ) (hn : n ≤ ℓ) (hℓ : 1 ≤ ℓ)
+    (hA : JEq Γ (.univ m) A A')
+    (hB : ∀ x ∉ L, JEq (Γ.cons x A) (.univ n) (B.open x) (B'.open x))
+    (hm : m ≤ ℓ) (hn : n ≤ ℓ) (hℓ : 1 ≤ ℓ)
   : JEq Γ (.univ (max m n)) (.pi A B) (.pi A' B')
   | abs {Γ : Ctx} {A A' : Tm 0} {B B' b b' : Tm 1} {t t' : Tm 1} {m n : ℕ} {L : Finset String}
-  (hA : JEq Γ (.univ m) A A')
-  (hB : ∀ x ∉ L, JEq (Γ.cons x A) (.univ n) (B.open x) (B'.open x))
-  (hb : ∀ x ∉ L, JEq (Γ.cons x A) (B.open x) (b.open x) (b'.open x))
-  : JEq Γ (A.pi B) (A.abs b) (A'.abs b')
+    (hA : JEq Γ (.univ m) A A')
+    (hB : ∀ x ∉ L, JEq (Γ.cons x A) (.univ n) (B.open x) (B'.open x))
+    (hb : ∀ x ∉ L, JEq (Γ.cons x A) (B.open x) (b.open x) (b'.open x))
+    : JEq Γ (A.pi B) (A.abs b) (A'.abs b')
   | app {Γ : Ctx} {A : Tm 0} {B : Tm 1} {f f' a a' Ba : Tm 0} {n : ℕ} {L : Finset String}
-  (hf : JEq Γ (A.pi B) f f')
-  (ha : JEq Γ A a a')
-  (hBa : JEq Γ (.univ n) (B.lst a) Ba)
-  : JEq Γ Ba (f.app a) (f'.app a')
+    (hf : JEq Γ (A.pi B) f f')
+    (ha : JEq Γ A a a')
+    (hBa : JEq Γ (.univ n) (B.lst a) Ba)
+    : JEq Γ Ba (f.app a) (f'.app a')
   -- Context well-formedness
   | nil_ok : JEq .nil .unit .null .null
   | cons_ok {Γ : Ctx} {x : String} {A : Tm 0} {ℓ}
-  (hΓ : JEq Γ .unit .null .null)
-  (hx : x ∉ Γ.dv)
-  (hA : JEq Γ (.univ ℓ) A A)
-  : JEq (Γ.cons x A) .unit .null .null
+    (hΓ : JEq Γ .unit .null .null)
+    (hx : x ∉ Γ.dv)
+    (hA : JEq Γ (.univ ℓ) A A)
+    : JEq (Γ.cons x A) .unit .null .null
   -- Reduction
   | beta_app {Γ : Ctx} {A : Tm 0} {B b : Tm 1} {a ba Ba : Tm 0} {n : ℕ} {L : Finset String}
-  (hf : JEq Γ (A.pi B) (A.abs b) (A.abs b))
-  (ha : JEq Γ A a a)
-  (hba : JEq Γ Ba (b.lst a) ba)
-  : JEq Γ Ba (.app (A.abs b) a) ba
+    (hf : JEq Γ (A.pi B) (A.abs b) (A.abs b))
+    (ha : JEq Γ A a a)
+    (hba : JEq Γ Ba (b.lst a) ba)
+    : JEq Γ Ba (.app (A.abs b) a) ba
   -- Reflexivity and extensionality
   | eqn_rfl {Γ : Ctx} {A a b: Tm 0} : JEq Γ A a b → JEq Γ (.univ 0) (.eqn a b) .unit
   | eqn_ext {Γ : Ctx} {A a b : Tm 0}
-  : JEq Γ A a a → JEq Γ A b b → JEq Γ (.univ 0) (.eqn a b) .unit → JEq Γ A a b
+    : JEq Γ A a a → JEq Γ A b b → JEq Γ (.univ 0) (.eqn a b) .unit → JEq Γ A a b
   -- Symmetry and transitivity
   | symm {Γ : Ctx} {A a b : Tm 0} : JEq Γ A a b → JEq Γ A b a
   | trans {Γ : Ctx} {A a b c : Tm 0}
-  (hab : JEq Γ A a b)
-  (hbc : JEq Γ A b c)
-  : JEq Γ A a c
+    (hab : JEq Γ A a b)
+    (hbc : JEq Γ A b c)
+    : JEq Γ A a c
   -- Casting
+  | cast_level {Γ : Ctx} {A A' : Tm 0} {ℓ : ℕ}
+    (hA : JEq Γ (.univ ℓ) A A')
+    : JEq Γ (.univ (ℓ + 1)) A A'
   | cast {Γ : Ctx} {A A' a a' : Tm 0} {ℓ : ℕ}
-  (hA : JEq Γ (.univ ℓ) A A')
-  (ha : JEq Γ A a a')
-  : JEq Γ A' a a'
+    (hA : JEq Γ (.univ ℓ) A A')
+    (ha : JEq Γ A a a')
+    : JEq Γ A' a a'
 
 def Ctx.WfEq (Γ : Ctx) (a b : Tm 0) : Prop := ∃A, JEq Γ A a b
 
@@ -70,16 +73,76 @@ theorem Ctx.TyEq.wf {Γ A B} (h : TyEq Γ A B) : WfEq Γ A B := have ⟨_, h⟩ 
 
 theorem Ctx.IsTy.wf {Γ A} (h : Ctx.IsTy Γ A) : Ctx.IsWf Γ A := TyEq.wf h
 
+def Ctx.IsSort (Γ : Ctx) (A : Tm 0) : Prop := ∃ℓ, TyEq Γ (.univ ℓ) A
+
 def Ctx.HasTy' (Γ : Ctx) (A : Tm 0) (a : Tm 0) : Prop := JEq Γ A a a
 
 theorem Ctx.JEq.lhs_ty' {Γ A a b} (h : JEq Γ A a b) : HasTy' Γ A a := h.trans h.symm
 
 theorem Ctx.JEq.rhs_ty' {Γ A a b} (h : JEq Γ A a b) : HasTy' Γ A b := h.symm.lhs_ty'
 
-def Ctx.Ok' (Γ : Ctx) : Prop := HasTy' Γ .unit .null
+theorem Ctx.JEq.ty_eq {Γ ℓ A B} (h : JEq Γ (.univ ℓ) A B) : TyEq Γ A B := ⟨ℓ, h⟩
+
+theorem Ctx.JEq.lhs_is_ty {Γ ℓ A B} (h : JEq Γ (.univ ℓ) A B) : IsTy Γ A := h.lhs_ty'.ty_eq
+
+theorem Ctx.JEq.rhs_is_ty {Γ ℓ A B} (h : JEq Γ (.univ ℓ) A B) : IsTy Γ B := h.rhs_ty'.ty_eq
 
 inductive Ctx.Ok : Ctx → Prop
   | nil : Ok .nil
   | cons {Γ : Ctx} {x : String} {A : Tm 0}
   (hΓ : Ok Γ) (hx : x ∉ Γ.dv) (hA : IsTy Γ A)
   : Ok (Γ.cons x A)
+
+theorem Ctx.JEq.ok {Γ A a b} (h : JEq Γ A a b) : Ok Γ := by
+  induction h <;> repeat first | assumption | constructor
+
+theorem Ctx.TyEq.ok {Γ A B} (h : TyEq Γ A B) : Ok Γ := have ⟨_, h⟩ := h; h.ok
+
+theorem Ctx.IsTy.ok {Γ A} (h : IsTy Γ A) : Ok Γ := TyEq.ok h
+
+theorem Ctx.JEq.null {Γ} (h : Ok Γ) : JEq Γ .unit .null .null := by
+  induction h with
+  | nil => exact .nil_ok
+  | cons _ _ hA => cases hA; constructor <;> assumption
+
+theorem Ctx.Ok.iff_null {Γ} : JEq Γ .unit .null .null ↔ Ok Γ := ⟨JEq.ok, JEq.null⟩
+
+def Ctx.Cmp (Γ : Ctx) (A a b : Tm 0) : Prop := HasTy' Γ A a ∧ HasTy' Γ A b
+
+theorem Ctx.Cmp.symm {Γ A a b} (h : Cmp Γ A a b) : Cmp Γ A b a
+  := ⟨h.right, h.left⟩
+
+theorem Ctx.Cmp.trans {Γ A a b c} (h : Cmp Γ A a b) (h' : Cmp Γ A b c) : Cmp Γ A a c
+  := ⟨h.left, h'.right⟩
+
+theorem Ctx.IsTy.univ {Γ ℓ} (h : Ok Γ) : IsTy Γ (.univ ℓ) := ⟨ℓ + 1, .univ (.null h)⟩
+
+theorem Ctx.IsTy.unit {Γ} (h : Ok Γ) : IsTy Γ .unit := ⟨0, .unit (.null h)⟩
+
+theorem Ctx.IsTy.empty {Γ} (h : Ok Γ) : IsTy Γ .empty := ⟨0, .empty (.null h)⟩
+
+theorem Ctx.JEq.cmp {Γ A a b} (h : JEq Γ A a b) : Cmp Γ A a b := ⟨h.lhs_ty', h.rhs_ty'⟩
+
+-- theorem Ctx.Ok.lookup {Γ x A} (h : Ok Γ) (hA : Lookup Γ x A) : IsTy Γ A := by
+--   induction hA <;> cases h
+
+--TODO: we need weakening!
+-- theorem Ctx.JEq.regular {Γ A a b} (h : JEq Γ A a b) : IsTy Γ A := by
+--   induction h with
+--   | fv => sorry
+--   | abs => sorry
+--   | app => sorry
+--   | nil_ok => sorry
+--   | cons_ok => sorry
+--   | cast hA => exact hA.rhs_is_ty
+--   | _ => first
+--     | assumption
+--     | constructor; constructor; apply JEq.null; apply IsTy.ok; assumption
+
+-- theorem Ctx.JEq.cast_cmp {Γ A B a b} (h : JEq Γ A a b) (h' : Cmp Γ B a b) : JEq Γ B a b := by
+--   induction h generalizing B with
+--   | fv => exact h'.left
+--   | univ => exact h'.left
+--   | eqn =>
+--     sorry
+--   | _ => sorry
